First verified version with dynamic allocation.

src/dafny/smart/DepositSmart.dfy
@@ -43,10 +43,9 @@ module DepositSmart {
     /**
      *  Provide deposit smart contract algorithms.
      */
-    class Deposit {
+    class {:autocontracts} Deposit {
 
         //  State Variables.
-        var a : seq<int>  
 
         /** The default value for the leaves. It is 0 in the orginal algorithm. */
         const d : int 
@@ -58,10 +57,14 @@ module DepositSmart {
         const TREE_HEIGHT : nat
 
         /** The values on the left siblings of the path to leaf at index k. */
-        var branch : seq<int>
+        ghost var rBranch : seq<int>
+
+        /** branch is rBranch in reverse order. */
+        var branch: array<int>
 
         /** The values of the right siblings of the path to leaf at index k. */
-        const zero_h : seq<int>
+        ghost const zero_h : seq<int>
+        const zero_hashes: array<int> 
 
         /** The number of values added to the list. Also the index of the next available leaf. */
         var count : nat 
@@ -76,25 +79,29 @@ module DepositSmart {
         /** 
          *  @note   `values` record the values added so far. buildMerkle(values, TREE_HEIGHT, f, d)
          *          is the Merkle tree that corresponds to `values`.
-         *          `branch` and `zero_h` should always contain the left (resp. right) siblings 
+         *          `rBranch` and `zero_h` should always contain the left (resp. right) siblings 
          *          of the path to the |values|-th leaf in the Merkle tree. 
          *  @note   |values| is the length of the
          *          list `values`.
          */
         predicate Valid()
-            reads this
+            // reads this, this.zero_hashes, this.branch
         {
             //  Constraints on height and length of lists.
-            1 <= TREE_HEIGHT == |branch| == |zero_h| 
+            1 <= TREE_HEIGHT == branch.Length == |rBranch| == |zero_h| 
+            && branch[..] == reverse(rBranch)
             //  Maximum number of values stored in the tree bounded.
             && count < power2(TREE_HEIGHT) 
             //  count is the number of values added so far and should correspond to |values|.
             && |values| == count
+            //  the pointers to the arrays are distinct
+            && zero_hashes != branch
             //  zero_h is constant and equal to default values for each level of t.
             && zero_h == zeroes(f, d, TREE_HEIGHT - 1)
-            //  branch and zero_h are the left and right siblings of path to 
+            && zero_hashes[..] == reverse(zero_h)
+            //  rBranch and zero_h are the left and right siblings of path to 
             //  |values|-th leaf in buildMerkle(values, TREE_HEIGHT, f, d)
-            && areSiblingsAtIndex(|values|, buildMerkle(values, TREE_HEIGHT, f, d), branch, zero_h)
+            && areSiblingsAtIndex(|values|, buildMerkle(values, TREE_HEIGHT, f, d), rBranch, zero_h)
         }
 
         /**
@@ -104,129 +111,118 @@ module DepositSmart {
          *  @param  f1      The function used to decorate the tree (e.g. hash).
          *  @param  default The default value of the leaves in the tree.
          *
-         *  @note           The initial value of `branch` is unconstrained (apart the length
+         *  @note           The initial value of `rBranch` is unconstrained (apart the length
          *                  that should be the same as `h`). This implies that the algorithms
-         *                  are correct given any initial values for `branch`.
+         *                  are correct given any initial values for `rBranch`.
          */
         constructor(h: nat, l : seq<int>, f1 : (int, int) -> int, default : int) 
             requires h >= 1
             requires |l| == h 
-            ensures Valid()
+            // ensures fresh({zero_hashes} - {this})
+            ensures fresh({branch, zero_hashes})
+            // ensures fresh({branch} - {this.zero_hashes, this})
+            // ensures Valid()
+            // ensures branch == reverse(rBranch)
         {
             //  State variables
             TREE_HEIGHT, count, f, d := h, 0, f1, default;
-            zero_h, branch := zeroes(f1, default, h - 1), l ;
+            zero_h, rBranch := zeroes(f1, default, h - 1), reverse(l) ;
+
+            // zero_hashes := reverse(zeroes(f1, default, h - 1));
+            zero_hashes := new int[h](i requires 0 <= i < h  => zeroes(f1, default, h - 1)[h - 1 - i]);
+            // init_zero_hashes(zero_hashes, h, f1, default);
+            // zero_hashes[0] := default;
+            // var i := 0;
+            // while i < h {
+            //     i := i + 1;
+            // }
+
+            // zero_hashes := init_zero_hashes(h, f1, default);
             // a := [];
             //  Ghost variables
+           
             values := [];
-            a := reverse(l);
+            branch := new int[h](i requires 0 <= i < h => l[i]);
             //  Proof that right siblings of path natToBitList2(0, h) are zero_h.
             bitToNatToBitsIsIdentity(0, h);
             valueIsZeroImpliesAllZeroes(natToBitList2(0, h));
             leafAtPathIsIntValueOfPath(natToBitList2(0, h), buildMerkle([], h, f1, default), 0, 0);
             rightSiblingsOfLastPathAreDefault(natToBitList2(0, h), buildMerkle([], h, f1, default), 0, f1, 0, default);
+            // assume(zero_hashes[..] == reverse(zero_h));
         }
 
-        ///////////////////////////////////////////////////////////////////////////
-        //  Functional versions of algorithms.
-        ///////////////////////////////////////////////////////////////////////////
+        // method init_zero_hashes(z: array<int>, h: nat, f1 : (int, int) -> int, d: int)
+        //     requires h >= 1
+        //     ensures z[..] == reverse(zeroes(f1, d, h - 1))
+        //     // modifies this.z
+        // {
+        //     // z := new int[h];
+        //     var i := 0 ;
+        //     z[0] := d;
+        //     while i < h - 1 {
+        //         z[i + 1] := f1(z[i], z[i]);
+        //         i := i + 1;
+        //     }
+        //     assume(z[..] == reverse(zeroes(f1, d, h - 1)));
+        // }
+        // for (uint height = 0; height < DEPOSIT_CONTRACT_TREE_DEPTH - 1; height++)
+        //     zero_hashes[height + 1] = sha256(abi.encodePacked(zero_hashes[height], zero_hashes[height]));
 
-        /**
-         *  The (almost) functional version deposit() function.
-         *
-         *  This method updates the left siblings (branch) in order
-         *  to maintain the correspondence with the Merkle tree for values.
-         *  This is captured by the Valid() predicate.
-         *  In this version we use the functions operating on sequences
-         *  in a functional style.
-         *  
-         *  @param  v   The new deposit amount.
-         */
-        method deposit_f(v : int) 
-            requires Valid()
-            requires count < power2(TREE_HEIGHT) - 1         
-            ensures Valid()
-            modifies this 
-        {
-            branch := computeLeftSiblingsOnNextpathWithIndex(TREE_HEIGHT, count, branch, zero_h, f, v);
-            count := count + 1;
-
-             //  Update ghost vars and prove correctness with new tree
-            computeNewLeftIsCorrect(values, v, TREE_HEIGHT, old(branch), zero_h, f, d);
-            values := values + [v];
-        }   
-
-        /**
-         *  The get_deposit_root() functional function.
-         *
-         *  This method should always return the root value of the tree.
-         *
-         *  @returns    The root value of the Merkle Tree for values.
-         */
-        method {:timeMultiplier 2} get_deposit_root_f() returns (r : int) 
-            requires Valid()
-            ensures Valid()
-            /** The result of get_deposit_root_() is the root value of the Merkle tree for values.  */
-            ensures r == buildMerkle(values, TREE_HEIGHT, f, d).v 
-            modifies {}
-        {
-            r := computeRootLeftRightUpWithIndex(TREE_HEIGHT, count, branch, zero_h, f, d);
-
-            calc ==> {
-                Valid();
-                |values| < power2(TREE_HEIGHT);
-            }
-            assert |values| < power2(TREE_HEIGHT) ;
-
-            //  The proof of post condition follows easily from:
-            computeRootIsCorrect(values, TREE_HEIGHT, branch, zero_h, f, d);
-        }
 
         ///////////////////////////////////////////////////////////////////////////
         //  Imperative versions of algorithms.
         ///////////////////////////////////////////////////////////////////////////
 
         /** 
-         *  This method updates the left siblings (branch) in order
+         *  This method updates the left siblings (rBranch) in order
          *  to maintain the correspondence with the Merkle tree for values.
          *  This is captured by the Valid() predicate.
          *  
          *  @param  v   The new deposit amount.
          */
          method {:timeLimitMultiplier 10} deposit(v : int) 
-            requires Valid()
+            // requires Valid()
             requires count < power2(TREE_HEIGHT) - 1         
-            ensures Valid()
-            modifies this 
+            // ensures Valid()
+            ensures values == old(values) + [v]
+            ensures count == old(count) + 1
+            modifies this, this.branch
         {
             var value := v;
             var size : nat := count;
             var i : nat := 0;
             
-            ghost var e := computeLeftSiblingsOnNextpathWithIndex(TREE_HEIGHT, old(size), old(branch), zero_h, f, v);
+            ghost var e := computeLeftSiblingsOnNextpathWithIndex(TREE_HEIGHT, old(size), old(rBranch), zero_h, f, v);
             ghost var p := natToBitList(|values|, TREE_HEIGHT);
            
-            //  In our version branch and zero_h store the vectors in reverse order, so we
+            //  In our version rBranch and zero_h store the vectors in reverse order, so we
             //  use TREE_HEIGHT - i - 1  instead of index i < TREE_HEIGHT in the original algorithm.
-            //  @todo   Add a copy of branch in reverse order to use index i.
+            //  @todo   Add a copy of rBranch in reverse order to use index i.
             //  Note that the test i < TREE_HEIGHT in the original
             //  version of the algorithm always evaluates to true and is redundant.
             while size % 2 == 1 
 
-                invariant branch == old(branch) 
+                invariant rBranch == old(rBranch) 
+                invariant zero_h == old(zero_h) 
+                invariant branch == old(branch)
+                invariant zero_hashes == old(zero_hashes)
+                invariant branch[..] == old(branch[..]) 
+                invariant zero_hashes[..] == old(zero_hashes[..])
+                invariant zero_hashes[..] == reverse(zero_h) 
+                invariant branch[..] == reverse(rBranch)
 
-                invariant 0 <= TREE_HEIGHT - i - 1 < |branch|
+                invariant 0 <= TREE_HEIGHT - i - 1 < |rBranch|
                 invariant 0 <= size < power2(TREE_HEIGHT - i) - 1
                 
-                invariant |branch| == |e| == |zero_h| == TREE_HEIGHT
+                invariant branch.Length == |rBranch| == |e| == |zero_h| == TREE_HEIGHT
 
                 //  Main invariant:
                 invariant e == 
                     computeLeftSiblingsOnNextpathWithIndex(
                         TREE_HEIGHT - i, size, 
-                        take(branch, TREE_HEIGHT - i), 
+                        take(rBranch, TREE_HEIGHT - i), 
                         take(zero_h, TREE_HEIGHT - i), f, value) 
-                    + drop(branch, TREE_HEIGHT - i)     //  proving the + may need sone help
+                    + drop(rBranch, TREE_HEIGHT - i)     //  proving the + may need sone help
 
                 //  Termination is easy as size decreases and must be zero.
                 decreases size 
@@ -235,74 +231,107 @@ module DepositSmart {
                 ghost var i' := TREE_HEIGHT - i;
                 ghost var v' := value;
                 ghost var s' := size / 2; 
+                assert(size < power2(i'));
+                assert(0 != size);
+                // assert(0 < size < power2(i'));
+                // calc < {
+                //     size;
+                //     power2(TREE_HEIGHT - i) - 1;
+                //     == calc == {
+                //         TREE_HEIGHT - i;
+                //         i';
+                //     }
+                //     == power2(i') - 1;
+                //     < power2(i');
+                // }
                 calc == {
                     e;
                     computeLeftSiblingsOnNextpathWithIndex(
                         TREE_HEIGHT - i, size, 
-                        take(branch, TREE_HEIGHT - i), 
+                        take(rBranch, TREE_HEIGHT - i), 
                         take(zero_h, TREE_HEIGHT - i), f, v') 
-                    + drop(branch, TREE_HEIGHT - i);
+                    + drop(rBranch, TREE_HEIGHT - i);
                     calc == {
                         TREE_HEIGHT - i;
                         i';
                     }
                     computeLeftSiblingsOnNextpathWithIndex(
                         i', size, 
-                        take(branch, i'), 
+                        take(rBranch, i'), 
                         take(zero_h, i'), f, v') 
-                    + drop(branch, i');
-                    { mainInvariantProofHelper(i', size, branch, zero_h, f, v'); }
+                    + drop(rBranch, i');
+                    { mainInvariantProofHelper(i', size, rBranch, zero_h, f, v'); }
                     computeLeftSiblingsOnNextpathWithIndex(
                         i' - 1, s', 
-                        take(branch, i' - 1), 
-                        take(zero_h, i' - 1), f,  f(branch[i' - 1], v')) 
-                    + drop(branch, i' - 1);
+                        take(rBranch, i' - 1), 
+                        take(zero_h, i' - 1), f,  f(rBranch[i' - 1], v')) 
+                    + drop(rBranch, i' - 1);
                 }
-
-                value := f(branch[TREE_HEIGHT - i - 1], value);
+                assert(rBranch[TREE_HEIGHT - i - 1] == branch[i]);
+                value := f(branch[i], value);
                 size := size / 2;
                 i := i + 1;
 
                 assert(s' == size);
                 assert(i' - 1 == TREE_HEIGHT - i);
-                assert(value == f(branch[i' - 1], v'));
+                assert(value == f(rBranch[i' - 1], v'));
                 
             }
-            //  Show that e == branch[TREE_HEIGHT - i - 1 := value]
+            //  Show that e == rBranch[TREE_HEIGHT - i - 1 := value]
             calc == {
                 e;
                 computeLeftSiblingsOnNextpathWithIndex(
                         TREE_HEIGHT - i, size, 
-                        take(branch, TREE_HEIGHT - i), 
+                        take(rBranch, TREE_HEIGHT - i), 
                         take(zero_h, TREE_HEIGHT - i), f, value) 
-                    + drop(branch, TREE_HEIGHT - i);
+                    + drop(rBranch, TREE_HEIGHT - i);
                 calc == {
                     computeLeftSiblingsOnNextpathWithIndex(
                         TREE_HEIGHT - i, size, 
-                        take(branch, TREE_HEIGHT - i), 
+                        take(rBranch, TREE_HEIGHT - i), 
                         take(zero_h, TREE_HEIGHT - i), f, value) ;
                     { assert(size % 2 == 0 && TREE_HEIGHT - i - 1 >= 0 ); }
-                    init(take(branch, TREE_HEIGHT - i)) + [value];
+                    init(take(rBranch, TREE_HEIGHT - i)) + [value];
                 }
-                init(take(branch, TREE_HEIGHT - i)) + [value] + drop(branch, TREE_HEIGHT - i);
-                { updateAndsplitSeqAtIndex(branch, value, TREE_HEIGHT - i);} 
-                branch[TREE_HEIGHT - i - 1 := value];
-                old(branch)[TREE_HEIGHT - i - 1 := value];
+                init(take(rBranch, TREE_HEIGHT - i)) + [value] + drop(rBranch, TREE_HEIGHT - i);
+                { updateAndsplitSeqAtIndex(rBranch, value, TREE_HEIGHT - i);} 
+                rBranch[TREE_HEIGHT - i - 1 := value];
+                old(rBranch)[TREE_HEIGHT - i - 1 := value];
             }
             //  This is the important hidden property: TREE_HEIGHT - i - 1 ( i < TREE_HEIGHT)
             //  in original version) is NEVER out of range, and always in [0, TREE_HEIGHT[
-            branch := branch[TREE_HEIGHT - i - 1 := value];
-            assert(branch == old(branch)[TREE_HEIGHT - i - 1 := value] == e);
-            
+            rBranch := rBranch[TREE_HEIGHT - i - 1 := value];
+
+            //  if follows that 0 <= i < |branch|
+            // branch := branch[i := value];
+            branch[i] := value;
+
+            assert(rBranch == old(rBranch)[TREE_HEIGHT - i - 1 := value] == e);
+            assert(branch[..] == old(branch[..])[i := value]);
+            assert(branch[..] == reverse(rBranch));
             //  Finally increment count. Note that count can be incremented at the beginning
             //  provided that the while loop condition is flipped to sizeA % 2 == 0.
             count := count + 1;
             //  Update values
             values := values + [v];
            
+           assert(areSiblingsAtIndex(|old(values)|, buildMerkle(old(values), TREE_HEIGHT, f, d), old(rBranch), zero_h));
             //  Use correctness lemma  
-            computeNewLeftIsCorrect(old(values), v, TREE_HEIGHT, old(branch), zero_h, f, d);
-
+        assert(zero_hashes[..] == old(zero_hashes[..]));
+        // assert(zero_h == old(zero_h) == zeroes(f, d, TREE_HEIGHT - 1));
+        // assert(values == old(values) + [v]);
+        assert(count == old(count) + 1 == |values| == |old(values)| + 1);
+        computeNewLeftIsCorrect(old(values), v, TREE_HEIGHT, old(rBranch), zero_h, f, d);
+        assert(areSiblingsAtIndex(|values|, buildMerkle(values, TREE_HEIGHT, f, d), rBranch, zero_h));
+        // assume(zero_h == zeroes(f, d, TREE_HEIGHT - 1));
+        // assume(1 <= TREE_HEIGHT == branch.Length == |rBranch| == |zero_h|);
+        // assume(branch[..] == reverse(rBranch));
+            //  Maximum number of values stored in the tree bounded.
+        // assume(count < power2(TREE_HEIGHT)); 
+            //  count is the number of values added so far and should correspond to |values|.
+        // assume(|values| == count);
+            //  zero_h is constant and equal to default values for each level of t.
+        // assume(zero_hashes[..] == old(zero_hashes[..]));
         }
 
         /**
@@ -373,19 +402,22 @@ module DepositSmart {
          *
          *  @returns    The root value of the Merkle Tree for values.
          */
-         method {:timeLimitMultiplier 6} get_deposit_root() returns (r : int) 
-            requires Valid()
-            ensures Valid()
+         method {:timeLimitMultiplier 8} get_deposit_root() returns (r : int) 
+            // requires Valid()
+            // requires branch == reverse(rBranch)
+            // ensures Valid()
+            // ensures branch == reverse(rBranch)
             /** The result of get_deposit_root_() is the root value of the Merkle tree for values.  */
             ensures r == buildMerkle(values, TREE_HEIGHT, f, d).v 
             modifies {}
+            // reads {this, this.branch}
         {
             //  Some help to prove that the main invariant holds on entry:
-            assert(take(branch, TREE_HEIGHT) == branch);
+            assert(take(rBranch, TREE_HEIGHT) == rBranch);
             assert(take(zero_h, TREE_HEIGHT) == zero_h);
 
             //  Store the expected result in a ghost variable.
-            ghost var e := computeRootLeftRightUpWithIndex(TREE_HEIGHT, count, branch, zero_h, f, d);
+            ghost var e := computeRootLeftRightUpWithIndex(TREE_HEIGHT, count, rBranch, zero_h, f, d);
 
             //  Start with default value for r.
             r := d;
@@ -401,20 +433,22 @@ module DepositSmart {
                 invariant e == 
                     computeRootLeftRightUpWithIndex(
                         TREE_HEIGHT - h, size, 
-                        take(branch, TREE_HEIGHT - h), take(zero_h, TREE_HEIGHT - h), f, r)
+                        take(rBranch, TREE_HEIGHT - h), take(zero_h, TREE_HEIGHT - h), f, r)
 
                 decreases TREE_HEIGHT - h 
             {
                 //  A little help for Dafny to check the proof:
-                assert(last(take(branch, TREE_HEIGHT - h)) == branch[TREE_HEIGHT - h - 1]);
+                assert(last(take(rBranch, TREE_HEIGHT - h)) == rBranch[TREE_HEIGHT - h - 1]);
                 assert(last(take(zero_h, TREE_HEIGHT - h)) == zero_h[TREE_HEIGHT - h - 1]);
-                assert(init(take(branch, TREE_HEIGHT - h)) == take(branch, TREE_HEIGHT - h - 1));
+                assert(init(take(rBranch, TREE_HEIGHT - h)) == take(rBranch, TREE_HEIGHT - h - 1));
                 assert(init(take(zero_h, TREE_HEIGHT - h)) == take(zero_h, TREE_HEIGHT - h - 1));
 
                 if size % 2 == 1 {
-                    r := f(branch[TREE_HEIGHT - h - 1], r);
+                    assert(rBranch[TREE_HEIGHT - h - 1] == branch[h]);
+                    r := f(branch[h], r);
                 } else {
-                    r := f(r, zero_h[TREE_HEIGHT - h - 1]);
+                    assert(zero_hashes[h] ==  zero_h[TREE_HEIGHT - h - 1]);
+                    r := f(r, zero_hashes[h]);
                 }
                 size := size / 2;
                 h := h + 1;
@@ -424,7 +458,7 @@ module DepositSmart {
             assert(e == computeRootLeftRightUpWithIndex(0, 0, [], [], f, r) == r);
 
             //  The proof of post condition follows easily from:
-            computeRootIsCorrect(values, TREE_HEIGHT, branch, zero_h, f, d);
+            computeRootIsCorrect(values, TREE_HEIGHT, rBranch, zero_h, f, d);
         }
 
     }
